\subsection{Perturbation Models}
The perturbation model would bring down the change in
temperature from exponent to the algebriac form. We have the first-order tayler
approximation of rate constant:
\begin{align*}
    k(\bar T + \delta T) &\approx k(\bar T) + \frac{E_a}{R\bar T^2} k(\bar T) \delta T\\
    \delta k &\approx p \bar k \delta T\\
    \text{Where,} \quad &\\
    p &= \frac{E_a}{RT_0^2}
\end{align*}
Introducing the above approximation into the lumped parameters from eqn.\ref{eqn::full_nonlinear}:
\begin{align*}
    f_{13} &= k_1 \quad&
    \implies \bar f_{13} &= \bar k_{1}, \quad&
    \delta f_{13} \delta T &= \lr{ p_{1} \bar k_{1} } \delta T\\
    %===
    f_{23} &= k_{4F} \quad &
    \implies \bar f_{23} &= \bar k_{4F}, \quad &
    \delta f_{23} \delta &= \lr{ p_{4F} \bar k_{4F} } \delta T\\
    %===
    f_{32} &= k_{4F} \Theta \quad &
    \implies \bar f_{32} &= \bar k_{4F} \Theta, \quad &
    \delta f_{32} \delta T &= \lr{ p_{32}  \bar k_{32} \Theta } \delta T
    \\
    f_{31} &= k_1 V \quad &
    \implies \bar f_{31} &= \bar k_1 V, \quad &
    \delta f_{31} \delta T &= \lr{ p_1 \bar k_1 V } \delta T
    \\
    f_{24} &= b_v F
    \quad &
    \implies \bar f_{24} &= b_v \bar F,
    \quad &
    \delta f_{24} \delta F &= b_v \delta F
    \\
    g_1    &= b_v F
    \quad &
    \implies \bar g_1 &= b_v \bar F,
    \quad &
    \delta g_1 \delta F &= b_v \delta F
    \\
    g_2    &= b_v F + k_{4F} \Theta
    \quad &
    \implies \bar g_2 &= b_v \bar F + \bar k_{4F} \Theta,
    \quad &
    \delta g_{2_F} \delta F + \delta g_{2_T} \delta T &= b_v \delta F +  \lr{ p_{32}  \bar k_{32}  \Theta } \delta T
    \\
    g_{3}  &= k_{4R}+k_3
    \quad &
    \implies \bar g_3 &= \bar k_{4R} + \bar k_3,
    \quad &
    \delta g_3 \delta T&= \lr{ p_{4R} \bar k_{4R} + p_3 \bar k_3} \delta T
    \\
    g_{23} &= k_{4R} b_v
    \quad &
    \implies \bar g_{23} &= \bar k_{4R} b_v,
    \quad &
    \delta g_{23} \delta T &= \lr{ p_{4R} \bar k_{4R} b_v } \delta T
    \\
    g_{32} &= k_{4F} V \Theta
    \quad &
    \implies \bar g_{32} &= \bar k_{4F} V \Theta,
    \quad &
    \delta g_{32} \delta T &= \lr{ p_{4F} \bar k_{4F} V \Theta } \delta T
    \\
    g_4 &= \omega_u
    \\
    b_{11} &= b_v F
    \quad &
    \implies \bar b_{11} &= b_v \bar F,
    \quad &
    \delta b_{11} \delta F &= b_v \delta F
    \\
    b_{42} &= \frac{\omega_u b_u}{F}
    \quad &
    \implies \bar b_{42} &= \frac{\omega_u b_u}{\bar F},
    \quad &
    \delta b_{42} \delta F &= -\lr{\frac{\omega_u b_u}{\bar F^2}} \delta F
\end{align*}


We have the purturbation models for individual state dynamics:
\begin{enumerate}
\item
\begin{align*}
    \dot x_1 &=  -f_{13}(T) x_1 x_3 -g_1(F) x_1 + b_{11}(F) u_1
    \\
    \implies
    \delta \dot x_1 &= \bm{-\lr{ \bar f_{13} \bar x_3 + \bar g_1 } &
                                    0 &
                                    -\bar f_{13} \bar x_1 &
                                    0
                        }
                    \bm{\delta x_1 \\ \delta x_2 \\ \delta x_3 \\ \delta x_4}
                    +
                        \bm{\bar b_{11} &
                            0 &
                            \delta f_{13} \bar x_1 \bar x_3 &
                            \lr{\delta b_{11} \bar u_1- \delta g_1 \bar x_1}
                        }
                    \bm{\delta u_1 \\ \delta u_2 \\ \delta T \\ \delta F}
\end{align*}
%===============================================================================
\item
\begin{align*}
\dot x_2 &= -g_2(F, T) x_2 + f_{23}(T) x_2 x_3 + g_{23}(T) x_3 + f_{24}(F) x_4 \\
\implies
\delta \dot x_2 &= \bm{0 &
                    \lr{ -\bar g_2 + \bar f_{23} \bar x_3 }&
                    \lr{\bar f_{23} \bar x_2 + \bar g_{23}}&
                    \bar f_{24}}
                    \bm{\delta x_1 \\ \delta x_2 \\ \delta x_3 \\ \delta x_4}
                    \\
                    &+
                    \bm{0&
                        0 &
                        \lr{-\delta g_{2_T} \bar x_2 + \delta f_{23} \bar x_2 \bar x_3 + \delta g_{23} \bar x_3} &
                        \lr{-\delta g_{2_F} \bar x_2 + \delta f_{24} \bar x_4 }
                        }
                    \bm{\delta u_1 \\ \delta u_2 \\ \delta T \\ \delta F}
\end{align*}
%===============================================================================
\item
\begin{align*}
\dot x_3 &= -f_{32}(T) x_2 x_3 -g_3(T) x_3 -f_{31}(T) x_1 x_3 + g_{32}(T) x_2 \\
\implies
\delta \dot x_3 &= \bm{-\bar f_{31} \bar x_3 &
                       -\bar f_{32} \bar x_3 + \bar g_{32} &
                       -\bar f_{32} \bar x_2 - \bar g_3 - \bar f_{31} \bar x_1 &
                       0}
                    \bm{\delta x_1 \\ \delta x_2 \\ \delta x_3 \\ \delta x_4}
                    \\
                    &+
                    \bm{0&
                        0&
                        -\delta f_{32} \bar x_2 \bar x_3 - \delta g_3 \bar x_3 - \delta f_{31} \bar x_1 \bar x_3 + \delta g_{32} \bar x_2 &
                        0}
                    \bm{\delta u_1 \\ \delta u_2 \\ \delta T \\ \delta F}
\end{align*}
%===============================================================================
\item
\begin{align*}
\dot x_4 &= -g_4 x_4 + b_{42}(F) u_2\\
\implies
\delta \dot x_4 &= \bm{0 & 0 & 0 & -g_4}
                    \bm{\delta x_1 \\ \delta x_2 \\ \delta x_3 \\ \delta x_4}
                    +
                    \bm{0&
                        \bar b_{42}&
                        0&
                        \delta b_{42} \bar u_2}
                    \bm{\delta u_1 \\ \delta u_2 \\ \delta T \\ \delta F}
\end{align*}
\end{enumerate}

Combining above equations, we have the linearised model of the system:

\begin{align*}
    \bm{\delta \dot x_1 \\ \delta \dot x_2 \\ \delta \dot x_3 \\ \delta \dot x_4} &= \bm{-\lr{ \bar f_{13} \bar x_3 + \bar g_1 } &
                    0 &
                    -\bar f_{13} \bar x_1 &
                    0 \\
                    %===
                    0 &
                    \lr{ -\bar g_2 + \bar f_{23} \bar x_3 }&
                    \lr{\bar f_{23} \bar x_2 + \bar g_{23}}&
                    \bar f_{24} \\
                    %===
                    -\bar f_{31} \bar x_3 &
                    \lr{-\bar f_{32} \bar x_3 + \bar g_{32} } &
                    \lr{-\bar f_{32} \bar x_2 - \bar g_3 - \bar f_{31} \bar x_1 } &
                    0 \\
                    %===
                    0 & 0 & 0 & -g_4
                    }
    \bm{\delta x_1 \\ \delta x_2 \\ \delta x_3 \\ \delta x_4}\\
            &\qquad+ \bm{ \bar b_{11} &
                            0 &
                            \delta f_{13} \bar x_1 \bar x_3 &
                            \lr{\delta b_{11} \bar u_1- \delta g_1 \bar x_1}
                            \\
                        %===
                        0&
                        0 &
                        \lr{-\delta g_{2_T} \bar x_2 + \delta f_{23} \bar x_2 \bar x_3 + \delta g_{23} \bar x_3} &
                        \lr{-\delta g_{2_F} \bar x_2 + \delta f_{24} \bar x_4 }
                        \\
                        %===
                        0&
                        0&
                        \lr{-\delta f_{32} \bar x_2 \bar x_3 - \delta g_3 \bar x_3 - \delta f_{31} \bar x_1 \bar x_3 + \delta g_{32} \bar x_2 } &
                        0
                        \\
                        %===
                        0&
                        \bar b_{42}&
                        0&
                        \delta b_{42} \bar u_2
                        }
    \bm{\delta u_1 \\ \delta u_2 \\ \delta T \\ \delta F}
\end{align*}
